\begin{proposition}
	If $ \mathcal{L}(\mathbf{\theta}) : \mathbb{R}^n \rightarrow \mathbb{R}$ $\mathbf{\theta} \mapsto  \mathcal{L}(\mathbf{\theta})=\frac{1}{m}\sum_{i=1}^m c_i+\mathbf{r}_i^T\mathbf{\theta}+\mathbf{\theta}^T\mathbf{Q}_i\mathbf{\theta}$ and $ c_i+\mathbf{r}_i^T\mathbf{\theta}+\mathbf{\theta}^T\mathbf{Q}_i\mathbf{\theta}= \BL[i](\mathbf{\theta})$ with $m$ being number the of batches $\mathbb{B}_i$. (Each batch defines a parabola. The empirical loss $\mathcal{L}(\mathbf{\theta})$ is the mean of these parabolas). And for all  $i,j \in \mathbb{N}$ it holds that $ \mathbf{Q}_i=\mathbf{Q}_j$ and that $\mathbf{Q_i}$ is positive definite. Then $\argmin{\theta} \mathcal{L}(\mathbf{\theta}) =\frac{1}{m}\sum_{i=1}^m\argmin{\theta} \BL[i](\mathbf{\theta})$ holds.
\end{proposition}

\begin{proof}
 \quad\\ 
 Since $\mathcal{L}(\mathbf{\theta})$ is a sum of convex functions, it is also convex and has one minimum.\\
 At first we determine the derivative of $\mathcal{L}(\mathbf{\theta})$ with respect to $\mathbf{\theta}$:
  \begin{equation}
 \frac{\partial}{\partial \mathbf{\theta}}\mathcal{L}(\mathbf{\theta})= \frac{1}{m}\sum\limits_{i=1}^m(\mathbf{r}_i+2\mathbf{Q}_i\mathbf{\theta})= 2\mathbf{Q}\mathbf{\theta}+\frac{1}{m}\sum\limits_{i=1}^m\mathbf{r}_i
 \end{equation}
% Let: 
% \begin{equation}
% 	\begin{aligned}
% 	\hat{\mathbf{\theta}} &= \argmin{\mathbf{\theta}} \mathcal{L}(\mathbf{\theta})\\
% 	\hat{\mathbf{t}} &= \argmin{\mathbf{t}} L(\mathbf{t})
% 	 \end{aligned}
% \end{equation}
Then we determine the minima:
   \begin{equation}
  \argmin{\mathbf{\theta}} \mathcal{L}(\mathbf{\theta}) \Leftrightarrow
 \frac{\partial}{\partial \mathbf{\theta}}\mathcal{L}(\mathbf{\theta}){=}\mathbf{0} \Leftrightarrow \mathbf{\theta}=-\frac{1}{2}( \sum\limits_{i=1}^m \mathbf{Q}_i)^{-1} \sum\limits_{i=1}^m \mathbf{r_i}= -\frac{1}{2m} \mathbf{Q}^{-1} \sum\limits_{i=1}^m \mathbf{r_i}
   \end{equation}
   \begin{equation}
\argmin{\mathbf{\theta}} \BL[i](\mathbf{\theta})=-\frac{1}{2}\mathbf{Q}^{-1}\mathbf{r}_i
 \end{equation}
 Thus, we get:
 \begin{equation}
  \argmin{\mathbf{\theta}} \mathcal{L}(\mathbf{\theta})= -\frac{1}{2m}\mathbf{Q}^{-1}\sum\limits_{i=1}^m \mathbf{r}_i=\frac{1}{m}\sum\limits_{i=1}^m -\frac{1}{2}\mathbf{Q}^{-1}\mathbf{r}_i =\frac{1}{m}\sum\limits_{i=1}^m\argmin{\mathbf{\theta}} \BL[i](\mathbf{\theta})
  \end{equation}
\end{proof}